AU_ind

ACTL/Car.v
@@ -2,84 +2,182 @@ Require Import ACTL.
 
 Set Implicit Arguments.
 
+Require Import Coq.Setoids.Setoid.
+
 
 
 Inductive state := State : bool -> bool -> bool  -> state.
 
-Inductive action := switch | brake | park.
+Inductive action := switch | brake | park | tau | isOn | isBraked | isParked.
+
 
 Inductive trans : state -> action -> state -> Prop :=
-| T_switchOn : trans (State false true true) switch (State true true true)
-| T_switchOff : trans (State true true true) switch (State false true true)
-| T_brake e b p : trans (State b e p) brake (State e (negb b) p)
-| T_park e b p : trans (State b e p) park (State e b (negb p)).
+    | Tr_SwitchOk e : trans (State e true true) switch (State (negb e) true true)
+    | Tr_SwitchNG e b p : andb b p = false -> trans (State e b p) switch (State e b p)
+    | Tr_Brake e b p : trans (State e b p) brake (State e (negb b) p)
+    | Tr_Park e b p : trans (State e b p) park (State e b (negb p))
+    | Tr_IsOn b p : trans (State true b p) isOn (State true b p)
+    | Tr_IsBraked e p : trans (State e true p) isBraked (State e true p)
+    | Tr_IsParked e b : trans (State e b true) isParked (State e b true)
+    | Tr_tau s: trans s tau s.
 
-
-
-Inductive var := isOn | isBraked | isParked.
-
-Definition valuation (v : var) (s : state) : Prop :=
-match s with 
-| State e b p =>
-    match v with 
-    | isOn => is_true e 
-    | isBraked => is_true b 
-    | isParked => is_true p 
-    end 
-end.
-
-Notation Path := (path state action trans).
-Notation Form := (form action var).
-Notation Formr := (formr action var).
-Check Path.
-
-Check atom.
-
-
-Notation IsOn := (atom _ _ isOn).
-Notation IsBraked := (atom _ _ isBraked).
-Notation IsParked := (atom _ _ isParked).
-
-Check action_.
-
-Notation Switch := (action_ _ switch).
-Notation Brake := (action_ _ brake).
-Notation Park := (action_ _ park).
-Check sat.
-
-Notation "|= f " := (forall s, sat state action trans var valuation f s).
-
-
-Theorem switch_restriction : 
-    |=  ((¬ IsOn ∧ IsBraked ∧ IsParked) → EX [Switch] IsOn).
+Theorem tau_eq s s' : trans s tau s' <->  s = s'.
 Proof.
-    intro.
-    unfold sat; intros.
-    inversion_clear H.
-    inversion_clear H0.
-    assert (s = State false true true).
-    {
-        destruct s.
-        simpl in *.
-        destruct b, b1, b0; auto;
-        try match goal with 
-        | [ H : ~ is_true true |- _] => contradiction H; unfold is_true; auto 
-        | [H : is_true false |- _] => inversion H
-        end. 
-    }
-    assert (trans s switch (State true true true))  by (rewrite H0; constructor).
-    Check nilp.
-    pose (p := nilp state action trans s switch (State true true true) H3).
-    pose (r := Run state action trans s p).
-    exists r; repeat split.
-    apply until_here; simpl; auto.
-    unfold r, nextStateOf; simpl.
-    rewrite H0; simpl.
+    split; intro H.
+    +   inversion H; subst; auto.
+    +   subst; constructor.
+Qed.       
+
+Notation "s |= f" := (@sat state action trans f s)(at level 80).
+Notation "|= f" := (forall s, s |= f)(at level 80).
+Notation τ := (action_ tau).
+Notation "< chi > f" := (E (⊤ [τ] U [chi] f))(at level 50, chi at level 5).
+Notation "[ chi ] f" := (¬ <chi> ¬ f)(at level 50, chi at level 5).
+Notation "'EX' f" := (<any> f)(at level 50).
+Notation "'AX' f" := ([any] f)(at level 50).
+Notation "'EF' f" := (f ∨ EF [any] f)(at level 50).
+Notation "'AF' f" := (f ∨ AF [any] f)(at level 50).
+Notation "'EG' f" := (¬ AF ¬ f)(at level 50).
+Notation "'AG' f" := (¬ EF ¬ f)(at level 50).
+
+Notation "f 'EU' f'" := (E (f U f'))(at level 50).
+
+
+Notation Path := (@path state action trans).
+Notation Form := (@form action).
+Notation Formr := (@formr action).
+
+
+
+
+Notation IsOn := (< (action_ isOn) > ⊤).
+Notation IsBraked := (<(action_ isBraked)> ⊤).
+Notation IsParked := (<(action_ isParked)> ⊤).
+
+Notation Switch := (action_ switch).
+Notation Brake := (action_ brake).
+Notation Park := (action_ park).
+
+Ltac  satisfy := unfold sat; fold (sat (trans := trans)).
+
+Definition engineState s :=
+    match s with 
+    | State b _ _ => b 
+    end.
+
+Definition brakeState s :=
+    match s with 
+    | State _ b _ => b 
+    end.
+
+Definition parkState s := 
+    match s with 
+    | State _ _ b => b
+    end.
+
+
+Theorem IsOn_spec s :
+    s |= IsOn <-> engineState s = true.
+Proof.
+    destruct s; simpl; split; satisfy; intro H.
+    +   induction H as [r [Hr [_ HU]]].
+        induction HU; simpl in *; auto; subst.
+        -   destruct r,p; simpl in *; subst; inversion t; auto.
+        -   apply IHHU; symmetry; apply tau_eq; auto.
+    +   subst.
+        remember (State true b0 b1).
+        assert (trans s isOn s) by (subst; constructor).
+        exists (Run s (nilp s isOn s H)); repeat split.
+        constructor; unfold sata; auto.
+Qed.   
+
+Theorem IsBraked_spec s :
+    s |= IsBraked <-> brakeState s = true.
+Proof.
+    destruct s; simpl; split; satisfy; intro H.
+    +   induction H as [r [Hr [_ HU]]].
+        induction HU; simpl in *; auto; subst.
+        -   destruct r,p; simpl in *; subst; inversion t; auto.
+        -   apply IHHU; symmetry; apply tau_eq; auto.
+    +   subst.
+        remember (State b true b1).
+        assert (trans s isBraked s) by (subst; constructor).
+        exists (Run s (nilp s isBraked s H)); repeat split.
+        constructor; unfold sata; auto.
+Qed.  
+
+Theorem IsParked_spec s :
+    s |= IsParked <-> parkState s = true.
+Proof.
+    destruct s; simpl; split; satisfy; intro H.
+    +   induction H as [r [Hr [_ HU]]].
+        induction HU; simpl in *; auto; subst.
+        -   destruct r,p; simpl in *; subst; inversion t; auto.
+        -   apply IHHU; symmetry; apply tau_eq; auto.
+    +   subst.
+        remember (State b b0 true).
+        assert (trans s isParked s) by (subst; constructor).
+        exists (Run s (nilp s isParked s H)); repeat split.
+        constructor; unfold sata; auto.
+Qed.
+
+
+    
+
+
+
+
+Theorem switch_safe : 
+    |= AG ((IsOn ∧ ¬ IsParked) → [Switch] IsOn).
+Proof.
+    satisfy; intros s F.
+    induction F.
+    +   apply imply_to_and in H.
+        induction H as [[H H0] H1].
+        apply IsOn_spec in H.
+        rewrite (IsParked_spec s) in H0.
+        assert (parkState s = false). 
+            { destruct (parkState s); auto. contradiction H0; auto. } 
+        clear H0.
+        apply NNPP in H1.
+        induction H1 as [r [Hr [_ HU]]].
+        induction HU.
+        -   apply H1; clear H1.
+            destruct s; simpl in *; subst.
+            destruct r, p; simpl in *; subst a s;
+                inversion t; subst;
+                remember (State true b0 false) as s;
+                assert (trans s isOn s); try( subst; constructor );
+                exists (Run s (nilp s isOn s H)); repeat split;
+                constructor; unfold sata; auto.
+        -   simpl in *; subst.
+            apply IHHU. symmetry. apply tau_eq; auto.
+    +   induction H as [r [Hr [_ HU]]]; subst.
+        induction HU; auto.
+        apply imply_to_and in H0.
+        induction H0 as [[H0 H1] H2].
+        apply IsOn_spec in H0.
+        rewrite (IsParked_spec (nextState r)) in H1.
+        assert (parkState (nextState r) = false).
+            { destruct r, p, s', b1; auto; contradiction H1; auto. }
+        clear H1.
+        apply NNPP in H2.
+        induction H2 as [r' [Hr' [_ HU']]].
+        induction HU'.
+        *   apply H2; clear H2.
+            destruct r,p; simpl in *; subst;
+            destruct r0; [destruct p| destruct p0]; simpl in *; subst;
+            destruct s0; simpl in *; subst; inversion t0; subst;
+                remember (State true b0 false) as s';
+                assert (trans s' isOn s') as H0; try (subst; constructor);
+                exists (Run s' (nilp s' isOn s' H0));
+                repeat split; constructor; unfold sata; auto.
+        *   apply IHHU'; simpl in *; subst.
+            symmetry; apply tau_eq; auto.
+Qed.
 
 
 
 
 
-
-
-
+      
